theories/segment_list.v
@@ -1,5 +1,6 @@
 From mathcomp Require Import ssreflect ssrbool eqtype seq.
 Require Import BinNat Lia.
+Require Export common.
 From Wasm Require Import numerics bytes memory.
 From stdpp Require Import gmap.
 
@@ -13,8 +14,8 @@ Record segment_list : Type := {
 
 
 Record allocator : Type := {
-    allocated : (* list (N * N * N) *) gmap N (N * N);
-    next_free : N;
+    allocated :  (* list (N * N * N) *) gmap N (N * N);
+    next_free : N; 
   }.
 
 
@@ -41,13 +42,30 @@ Definition count_some (x : N) l :=
                     | Some y => if (y =? x)%N then acc + 1 else acc
                     | None => acc end) l 0. *) 
 
+(* Lemma decision_equal_first nid :
+  forall (x: N * N * N), Decision (let '(n, _, _) := x in n = nid).
+Proof. intros [[??]?]. unfold Decision. decidable_equality. Qed. *)
+
+(*Definition find (nid : N) (l : list (N * N * N)) : option (N * N) :=
+  match partition (fun '(n, _, _) => (n =? nid)%N) l with
+  | ([ (_,b,c) ], _) => Some (b, c)
+  | _ => None
+  end.
+
+
+Definition find_and_remove (nid : N) (l : list (N * N * N)): option (list (N * N * N) * N * N) :=
+  match partition (fun '(n, _, _) => (n =? nid)%N) l with 
+  | ([ (_,b,c) ], l) => Some (l, b, c)
+  | _ => None
+  end. *)
+
 Definition find (nid : N) (l : gmap N (N * N)) : option (N * N) :=
   l !! nid.
 Definition find_and_remove (nid : N) (l : gmap N (N * N)) : option (gmap N (N * N) * N * N) :=
   match l !! nid with
   | Some (b, c) => Some (delete nid l, b, c)
   | None => None
-  end. 
+  end.  
 
 (*
 Fixpoint find (nid : N) (l: list (N * N * N)) : option (N * N) :=
@@ -94,9 +112,9 @@ Definition isFree nid s : Prop :=
 (*  s.(allocated) !! nid = None.*) find nid s.(allocated) = None. 
 
 
-Definition compatible addr size (s : gmap N (N * N)) : Prop :=
+ Definition compatible addr size (s : gmap N (N * N)) : Prop :=
   forall nid addr' size', s !! nid = Some (addr', size') ->
-                     (addr + size <= addr')%N \/ (addr >= addr' + size')%N.
+                     (addr + size <= addr')%N \/ (addr >= addr' + size')%N. 
 (*
 Fixpoint compatible addr size (l : list (N * N * N)) : Prop :=
   match l with
@@ -118,10 +136,11 @@ Proof.
     apply (H (n2, n3, n4)).
     by right.
 Qed. 
+
+
 *)
 
-
-(*  
+ (*
 Fixpoint fresh_nid_aux (l : list (N * N * N)) :=
   match l with
   | [::] => 0%N
@@ -129,19 +148,21 @@ Fixpoint fresh_nid_aux (l : list (N * N * N)) :=
                     if (x <=? id)%N then (id + 1)%N else x
   end.
 
-Definition fresh_nid A := fresh_nid_aux A.(allocated). *)
-(*
+Definition fresh_nid A := fresh_nid_aux A.(allocated). 
+
 Lemma fresh_nid_is_free_aux: forall l n, (n >= fresh_nid_aux l)%N -> isFree n {| allocated := l |}.
 Proof.
   induction l; intros => //=.
   simpl in H. destruct a. destruct p.
   unfold isFree. simpl.
+  unfold find. simpl.
   destruct (n1 =? n)%N eqn:Hn'.
   apply N.eqb_eq in Hn' as ->.
   destruct (fresh_nid_aux l <=? n)%N eqn:Hn; [ lia | apply N.leb_gt in Hn; lia].
   assert (n >= fresh_nid_aux l)%N as H0; last first.
   apply IHl in H0.
-  unfold isFree in H0. simpl in H0. done.
+  unfold isFree in H0. unfold find in H0. simpl in H0.
+  destruct (partition _ l) eqn:Hl. done. 
   destruct (fresh_nid_aux l <=? n1)%N eqn:Hn; last done.
   apply N.leb_le in Hn. lia.
 Qed. 
@@ -153,8 +174,8 @@ Proof.
   intro A. destruct A. unfold fresh_nid. apply fresh_nid_is_free_aux.
   simpl. lia.
 Qed. 
-  
-*)
+  *)
+
 (*
 Lemma fresh_nid: forall A, exists nid, forall nid', (nid' >= nid)%N -> isFree nid' A.
 Proof.
@@ -223,20 +244,20 @@ Definition seg_grow :=
 (* Definition isSound_aux T (l : list (N * N * N)) : Prop :=
   List.forallb (fun '(a,b,c) => N.leb (b + c) (seg_length T)) l. *)
 
-Definition isSound_aux T (m : gmap N (N * N)) : Prop :=
+ Definition isSound_aux T (m : gmap N (N * N)) : Prop :=
   forall a b c, m !! a = Some (b,c) ->
-           (b + c <= seg_length T)%N /\ compatible b c (delete a m).
+           (b + c <= seg_length T)%N /\ compatible b c (delete a m). 
 (*
 Fixpoint isSound_aux T (l : list (N * N * N)) : Prop :=
   match l with
   | [::] => True
   | (a,b,c) :: q => N.leb (b + c) (seg_length T) /\ compatible b c q /\
                     ~(List.In a (List.map (fun '(x,_,_) => x) q)) /\ isSound_aux T q
-  end.  *)
+  end. *)
 
-Definition isSound T A : Prop :=
+ Definition isSound T A : Prop :=
   isSound_aux T A.(allocated) /\
-    forall k, (k >= A.(next_free))%N -> A.(allocated) !! k = None.
+    forall k, (k >= A.(next_free))%N -> A.(allocated) !! k = None.  
 
 
 
@@ -248,9 +269,8 @@ Proof.
   intros a b c Ha.
   apply Hsound in Ha.
   right. lia.
-Qed.
-(*
-  intro l. induction l => //=.
+Qed. 
+(*  intro l. induction l => //=.
   intros. destruct a. destruct p.
   destruct H as (Hlim & Hcomp & Hdup & H).
   split.
@@ -258,8 +278,8 @@ Qed.
     apply N.leb_le in Hlim. lia.
   - apply IHl.
     done. 
-Qed. 
-*)
+Qed.  *)
+
 
 Lemma data_length_is_compatible :
   forall T A size, isSound T A -> compatible (seg_length T) size A.(allocated).
@@ -269,6 +289,17 @@ Proof.
   by destruct H.
 Qed.
 
+(*
+Lemma partition_all_true {A} f (l: list A): forall l', partition f l = (l', []) -> l = l'.
+Proof. induction l => //=. intros * H; by inversion H.
+       destruct (partition f l). destruct (f a) => //.
+       intros * H; inversion H; subst. by erewrite IHl. Qed.
+
+Lemma partition_all_false {A} f (l: list A): forall l', partition f l = ([], l') -> l = l'.
+Proof. induction l => //=. intros * H; by inversion H.
+       destruct (partition f l). destruct (f a) => //.
+       intros * H; inversion H; subst. by erewrite IHl. Qed.
+  *)    
 
 Lemma find_and_remove_compatible:
   forall l nid l' a n add size,
@@ -288,11 +319,13 @@ Proof.
     rewrite lookup_delete_ne in Hnid' => //.
     by apply Hcomp in Hnid'.
 Qed.
-(*  
-  induction l => //=.
+(*  induction l => //=.
   intros * Hcomp Hfr. destruct a as [[??]?].
+  unfold find_and_remove in Hfr. simpl in Hfr.
+  destruct (partition _ l) eqn:Hl.
   destruct (n0 =? nid)%N.
-  - inversion Hfr; subst. by destruct Hcomp.
+  - destruct l0; inversion Hfr; subst.
+    apply partition_all_false in Hl by destruct Hcomp.
   - destruct Hcomp as [??]. destruct (find_and_remove nid l) eqn:Hfr' => //.
     destruct p as [[??]?]. eapply IHl in Hfr' => //; last exact H0.
     inversion Hfr; subst. simpl. split => //.
