theories/iris/language/iris_wp_def.v
@@ -42,13 +42,19 @@ Class wasmG Σ :=
 
       memlimit_hsG :> gen_heapGS N (option N) Σ;
 
-      seg_gen_hsG :> gen_heapGS N (byte * btag) Σ;
+      (*      seg_gen_hsG :> gen_heapGS N (byte * btag) Σ; *)
+      segGName : gname;
+
+      seg_gen_hsG :> ghost_mapG Σ N (byte * btag);
 
       segsize_gen_hsG :> gen_heapGS unit N Σ;
 
       seglimit_hsG :> gen_heapGS unit (option N) Σ;
 
-      alloc_gen_hsG :> gen_heapGS N (N*N) Σ;
+      (*      alloc_gen_hsG :> gen_heapGS N (N*N) Σ; *)
+      allGName : gname;
+
+      all_gen_hsG :> ghost_mapG Σ N (N * N);
 
       glob_gen_hsG :> gen_heapGS N global Σ;
 
@@ -78,8 +84,8 @@ Definition gen_heap_wasm_store `{!wasmG Σ} (s: store_record) : iProp Σ :=
   ((gen_heap_interp (gmap_of_list s.(s_funcs))) ∗
    (gen_heap_interp (gmap_of_table s.(s_tables))) ∗
    (gen_heap_interp (gmap_of_memory s.(s_mems))) ∗
-   (gen_heap_interp (gmap_of_segment s.(s_segs))) ∗
-   (gen_heap_interp (gmap_of_allocator s.(s_alls))) ∗
+(*   (gen_heap_interp (gmap_of_segment s.(s_segs) s.(s_alls))) ∗ *)
+(*   (gen_heap_interp (gmap_of_allocator s.(s_alls))) ∗ *)
    (gen_heap_interp (gmap_of_list s.(s_globals))) ∗
    (gen_heap_interp (gmap_of_list (fmap mem_length s.(s_mems)))) ∗
    (gen_heap_interp ({[ () := seg_length s.(s_segs).(seg_data)]} : gmap unit N)) ∗
@@ -95,8 +101,10 @@ Global Instance heapG_irisG `{!wasmG Σ} : irisGS wasm_lang Σ := {
      ((gen_heap_interp (gmap_of_list s.(s_funcs))) ∗
       (gen_heap_interp (gmap_of_table s.(s_tables))) ∗
       (gen_heap_interp (gmap_of_memory s.(s_mems))) ∗
-      (gen_heap_interp (gmap_of_segment s.(s_segs))) ∗
-      (gen_heap_interp (gmap_of_allocator s.(s_alls))) ∗
+      (*      (gen_heap_interp (gmap_of_segment s.(s_segs) s.(s_alls))) ∗ *)
+      (ghost_map_auth segGName 1 (gmap_of_segment s.(s_segs) s.(s_alls))) ∗
+      (*      (gen_heap_interp (gmap_of_allocator s.(s_alls))) ∗ *)
+      (ghost_map_auth allGName 1 (gmap_of_allocator s.(s_alls))) ∗
       (gen_heap_interp (gmap_of_list s.(s_globals))) ∗
       (ghost_map_auth frameGName 1 (<[ tt := Build_frame locs inst ]> ∅)) ∗ 
       (gen_heap_interp (gmap_of_list (fmap mem_length s.(s_mems)))) ∗
@@ -139,18 +147,27 @@ Notation "n ↦[wmlength] v" := (mapsto (L:=N) (V:=N) n (DfracOwn 1) v% V)
                            (at level 20, format "n ↦[wmlength] v") : bi_scope.
 Notation "n ↪[wmlimit] v" := (mapsto (L:=N) (V:=option N) (hG:=memlimit_hsG) n (DfracDiscarded) v% V)
                                (at level 20, format "n ↪[wmlimit] v") : bi_scope.
-Notation " ↦[ws]{ q } [ i ] v" := (mapsto (L:=N) (V:=byte * btag) i q v%V)
+(*Notation " ↦[ws]{ q } [ i ] v" := (mapsto (L:=N) (V:=byte * btag) i q v%V)
                                     (at level 20, q at level 5, format " ↦[ws]{ q } [ i ] v"): bi_scope.
 Notation " ↦[ws][ i ] v" := (mapsto (L:=N) (V:= byte * btag) i (DfracOwn 1) v%V)
+                              (at level 20, format " ↦[ws][ i ] v"): bi_scope. *)
+Notation " ↦[ws]{ q }[ i ] v" := (ghost_map_elem segGName i q v)
+                                   (at level 20, q at level 5, format " ↦[ws]{ q }[ i ] v") : bi_scope.
+Notation " ↦[ws][ i ] v" := (ghost_map_elem segGName i (DfracOwn 1) v)
                               (at level 20, format " ↦[ws][ i ] v"): bi_scope.
 Notation " ↦[wslength] v" := (mapsto (L:=unit) (V:=N) () (DfracOwn 1) v%V)
                                (at level 20, format " ↦[wslength] v"): bi_scope.
 Notation " ↪[wslimit] v" := (mapsto (L:=unit) (V:=option N) (hG:=seglimit_hsG) () (DfracDiscarded) v % V)
                               (at level 20, format " ↪[wslimit] v") : bi_scope.
-Notation "n ↣[allocated]{ q } v" := (mapsto (L:=N) (V:=N*N) n q v%V)
+(* Notation "n ↣[allocated]{ q } v" := (mapsto (L:=N) (V:=N*N) n q v%V)
                                       (at level 20, q at level 5, format "n ↣[allocated]{ q } v") : bi_scope.
 Notation "n ↣[allocated] v" := (mapsto (L:=N) (V:=N*N) n (DfracOwn 1) v%V)
+                                 (at level 20, format "n ↣[allocated] v") : bi_scope. *)
+Notation "n ↣[allocated]{ q } v" := (ghost_map_elem allGName n q v)
+                                      (at level 20, q at level 5, format "n ↣[allocated]{ q } v") : bi_scope.
+Notation "n ↣[allocated] v" := (ghost_map_elem allGName n (DfracOwn 1) v)
                                  (at level 20, format "n ↣[allocated] v") : bi_scope.
+
 Notation "n ↦[wg]{ q } v" := (mapsto (L:=N) (V:=global) n q v%V)
                            (at level 20, q at level 5, format "n ↦[wg]{ q } v").
 Notation "n ↦[wg] v" := (mapsto (L:=N) (V:=global) n (DfracOwn 1) v%V)
